fol/src/FOLAPI.v
@@ -1,21 +1,48 @@
 Require Import Coq.Strings.String.
 Require Import Coq.ZArith.BinInt.
 Require Import Coq.Lists.List.
+Require Import Coq.Bool.Bool.
 Import ListNotations.
 Local Open Scope Z_scope.
+From CoqCompat Require CoqBigInt.
+From CoqCompat Require Import Monads CoqCtr.
 
 (*Every term variable has type int*)
 
 (*Variables*)
-Definition var : Set := string.
+Definition var : Set := (string * CoqBigInt.t)%type.
+
+Definition var_eqb (v1 v2: var) : bool :=
+  (*Compare tags first*)
+  CoqBigInt.eqb (snd v1) (snd v2) &&
+  String.eqb (fst v1) (fst v2).
+
+(*Want in [Prop], not [reflect]*)
+Lemma var_eqb_eq v1 v2: var_eqb v1 v2 = true <-> v1 = v2.
+Proof.
+  unfold var_eqb. rewrite andb_true_iff, CoqBigInt.eqb_eq, String.eqb_eq.
+  destruct v1 as [s1 i1]; destruct v2 as [s2 i2]; simpl; split;
+  intros Heq; inversion Heq; subst; auto.
+Qed.
+
+Definition var_dec (v1 v2: var) : {v1 = v2} + {v1 <> v2}.
+Proof.
+  destruct (var_eqb v1 v2) eqn : Hvar.
+  - left. apply var_eqb_eq in Hvar; auto.
+  - right. intro Hc. subst. 
+    assert (Hvar2: var_eqb v2 v2 = true) by (apply var_eqb_eq; auto).
+    rewrite Hvar in Hvar2. discriminate.
+Defined.
 
 (*Terms*)
 Unset Elimination Schemes.
+
+Variant intop := | Add | Mult.
+
 Inductive tm := 
 | Tconst: Z -> tm
 | Tvar: var -> tm
-| Tadd: tm -> tm -> tm
-| Tmult: tm -> tm -> tm
+| Top: intop -> tm -> tm -> tm
 | Tlet: tm -> (var * tm) -> tm.
 
 (*Boolean operators*)
@@ -44,16 +71,14 @@ Section TermInd.
 Variable (P: tm -> Prop) 
 (Pconst: forall c, P (Tconst c))
 (Pvar: forall v, P (Tvar v))
-(Padd: forall t1 t2, P t1 -> P t2 -> P (Tadd t1 t2))
-(Pmult: forall t1 t2, P t1 -> P t2 -> P (Tmult t1 t2))
+(Pop: forall o t1 t2, P t1 -> P t2 -> P (Top o t1 t2))
 (Plet: forall t1 b, P t1 -> P (snd b) -> P (Tlet t1 b)).
 
 Fixpoint tm_ind (t: tm) : P t :=
   match t with
   | Tconst c => Pconst c
   | Tvar v => Pvar v
-  | Tadd t1 t2 => Padd _ _ (tm_ind t1) (tm_ind t2)
-  | Tmult t1 t2 => Pmult _ _ (tm_ind t1) (tm_ind t2)
+  | Top o t1 t2 => Pop o _ _ (tm_ind t1) (tm_ind t2)
   | Tlet t1 (v, t2) => Plet _ (v, t2) (tm_ind t1) (tm_ind t2)
   end.
 End TermInd.
@@ -86,13 +111,13 @@ End FmlaInd.
 (*Variable valuation*)
 Definition val := var -> Z.
 Definition add_val (x: var) (z: Z) (v: val) : val :=
-  fun y => if string_dec x y then z else v y.
+  fun y => if var_dec x y then z else v y.
 
 Lemma add_val_twice (x : var) (z1 z2: Z) (v: val):
 forall p,
   add_val x z1 (add_val x z2 v) p = add_val x z1 v p.
 Proof.
-  intros p. unfold add_val. destruct (string_dec x p); subst; auto.
+  intros p. unfold add_val. destruct (var_dec x p); subst; auto.
 Qed.
 
 Lemma add_val_switch (x y : var) (z1 z2: Z) (v: val):
@@ -101,16 +126,21 @@ Lemma add_val_switch (x y : var) (z1 z2: Z) (v: val):
   add_val x z1 (add_val y z2 v) p = add_val y z2 (add_val x z1 v) p.
 Proof.
   intros Hxy p. unfold add_val.
-  destruct (string_dec x p); subst; auto.
-  destruct (string_dec y p); subst; auto.
+  destruct (var_dec x p); subst; auto.
+  destruct (var_dec y p); subst; auto.
   contradiction.
 Qed.
+
+Definition intop_rep (o: intop) : Z -> Z -> Z :=
+  match o with
+  | Add => Z.add
+  | Mult => Z.mul
+  end.
 
 Fixpoint tm_rep (v: val) (t: tm) : Z :=
   match t with
   | Tvar x => v x
-  | Tadd t1 t2 => (tm_rep v t1) + (tm_rep v t2)
-  | Tmult t1 t2 => (tm_rep v t1) * (tm_rep v t2)
+  | Top o t1 t2 => intop_rep o (tm_rep v t1) (tm_rep v t2)
   | Tconst c => c
   | Tlet t1 (x, t2) => tm_rep (add_val x (tm_rep v t1) v) t2
   end.
@@ -138,12 +168,11 @@ Fixpoint fmla_rep (v: val) (f: fmla) : Prop :=
 (*First, unsafe substitutiuon*)
 Fixpoint tm_subst_unsafe (v: var) (t: tm) (t1: tm) : tm :=
   match t1 with
-  | Tvar x => if string_dec v x then t else t1
+  | Tvar x => if var_dec v x then t else t1
   | Tconst c => Tconst c
-  | Tadd t1 t2 => Tadd (tm_subst_unsafe v t t1) (tm_subst_unsafe v t t2)
-  | Tmult t1 t2 => Tmult (tm_subst_unsafe v t t1) (tm_subst_unsafe v t t2)
+  | Top o t1 t2 => Top o (tm_subst_unsafe v t t1) (tm_subst_unsafe v t t2)
   | Tlet t1 (y, t2) => Tlet (tm_subst_unsafe v t t1) 
-    (y, (if string_dec v y then t2 else tm_subst_unsafe v t t2))
+    (y, (if var_dec v y then t2 else tm_subst_unsafe v t t2))
   end.
 Fixpoint fmla_subst_unsafe (v: var) (t: tm) (f: fmla) : fmla :=
   match f with
@@ -152,9 +181,9 @@ Fixpoint fmla_subst_unsafe (v: var) (t: tm) (f: fmla) : fmla :=
   | Fbinop b f1 f2 => Fbinop b (fmla_subst_unsafe v t f1) (fmla_subst_unsafe v t f2)
   | Fnot f => Fnot (fmla_subst_unsafe v t f)
   | Fforall (x, f) => 
-    Fforall (x, if string_dec v x then f else fmla_subst_unsafe v t f)
+    Fforall (x, if var_dec v x then f else fmla_subst_unsafe v t f)
   | Fexists (x, f) => 
-    Fexists (x, if string_dec v x then f else fmla_subst_unsafe v t f)
+    Fexists (x, if var_dec v x then f else fmla_subst_unsafe v t f)
   end.
 
 (*Free variables*)
@@ -162,9 +191,8 @@ Fixpoint tm_fv (t: tm) : list var :=
   match t with
   | Tvar x => [x]
   | Tconst _ => nil
-  | Tadd t1 t2 => tm_fv t1 ++ tm_fv t2
-  | Tmult t1 t2 => tm_fv t1 ++ tm_fv t2
-  | Tlet t1 (x, t2) => tm_fv t1 ++ (remove string_dec x (tm_fv t2))
+  | Top _ t1 t2 => tm_fv t1 ++ tm_fv t2
+  | Tlet t1 (x, t2) => tm_fv t1 ++ (remove var_dec x (tm_fv t2))
   end.
 Fixpoint fmla_fv (f: fmla) : list var :=
   match f with
@@ -172,10 +200,26 @@ Fixpoint fmla_fv (f: fmla) : list var :=
   | Flt t1 t2 => tm_fv t1 ++ tm_fv t2
   | Fbinop _ f1 f2 => fmla_fv f1 ++ fmla_fv f2
   | Fnot f => fmla_fv f
-  | Fforall (x, f) => remove string_dec x (fmla_fv f)
-  | Fexists (x, f) => remove string_dec x (fmla_fv f)
+  | Fforall (x, f) => remove var_dec x (fmla_fv f)
+  | Fexists (x, f) => remove var_dec x (fmla_fv f)
   end.
 
+(*Bound variables*)
+Fixpoint tm_bnd (t: tm) : list var :=
+  match t with
+  | Tlet t1 (x, t2) => x :: (tm_bnd t1) ++ (tm_bnd t2)
+  | Top _ t1 t2 => tm_bnd t1 ++ tm_bnd t2
+  | _ => nil
+  end.
+Fixpoint fmla_bnd (f: fmla) : list var :=
+  match f with
+  | Feq t1 t2 => tm_bnd t1 ++ tm_bnd t2
+  | Flt t1 t2 => tm_bnd t1 ++ tm_bnd t2
+  | Fbinop _ f1 f2 => fmla_bnd f1 ++ fmla_bnd f2
+  | Fnot f => fmla_bnd f
+  | Fforall (x, f) => x :: fmla_bnd f
+  | Fexists (x, f) => x :: fmla_bnd f
+  end.
 
 (*Semantics for unsafe substitution*)
 
@@ -184,11 +228,11 @@ Lemma tm_rep_change_vv (t: tm):
   forall (vv1 vv2: val) (Hvv: forall x, In x (tm_fv t) -> vv1 x = vv2 x),
   tm_rep vv1 t = tm_rep vv2 t.
 Proof.
-  induction t as [| | t1 t2 IH1 IH2 | t1 t2 IH1 IH2 | t1 [x t2] IH1 IH2]; simpl; auto;
+  induction t as [| | o t1 t2 IH1 IH2 | t1 [x t2] IH1 IH2]; simpl; auto;
   intros vv1 vv2 Hvv; try (setoid_rewrite in_app_iff in Hvv);
   rewrite (IH1 vv1 vv2); auto; try solve[f_equal; auto].
   apply IH2; simpl. intros y Hiny.
-  unfold add_val. destruct (string_dec x y); subst; auto.
+  unfold add_val. destruct (var_dec x y); subst; auto.
   apply Hvv. right. apply in_in_remove; auto.
 Qed.
 
@@ -212,61 +256,1262 @@ Proof.
     reflexivity];
   (*last 2 cases*)
   try solve[setoid_rewrite IH; [reflexivity | |]; auto; simpl;
-    intros y Hiny; unfold add_val; destruct (string_dec x y); subst; auto;
+    intros y Hiny; unfold add_val; destruct (var_dec x y); subst; auto;
     symmetry; apply Hvv, in_in_remove; auto].
   apply binop_rep_congr; auto.
 Qed.
 
-(*TODO START: define tm_bnd*)
 Lemma tm_subst_unsafe_rep (v: var) (t: tm) (t1: tm) :
-  (forall x, In x (tm_fv t) -> ~ In x (tm_bnd t1)) ->
+  (*Ensure no capture: no variable free in t can be bound in t1*)
+  (forall x, In x (tm_fv t) -> In x (tm_bnd t1) -> False) ->
   forall (vv: val), tm_rep vv (tm_subst_unsafe v t t1) =
   tm_rep (add_val v (tm_rep vv t) vv) t1.
 Proof.
-  induction t1 as [| x | | | t1 [x t2] IH1 IH2]; simpl; auto; intros vv;
-  try solve[f_equal; auto].
-  - (*var*) unfold add_val. destruct (string_dec v x); auto.
-  - (*let*) rewrite <- IH1.
-    destruct (string_dec v x); subst; auto.
+  induction t1 as [| x | o t1 t2 IH1 IH2 | t1 [x t2] IH1 IH2]; simpl; auto; intros Hbnd vv;
+  try solve[setoid_rewrite in_app_iff in Hbnd; f_equal; eauto].
+  - (*var*) unfold add_val. destruct (var_dec v x); auto.
+  - (*let*) setoid_rewrite in_app_iff in Hbnd. rewrite <- IH1 by eauto.
+    destruct (var_dec v x); subst; auto.
     + apply tm_rep_change_vv. intros y Hy.
-      unfold add_val. destruct (string_dec x y); auto.
+      unfold add_val. destruct (var_dec x y); auto.
     + simpl in IH2.
-      rewrite IH2.
+      rewrite IH2 by eauto.
       apply tm_rep_change_vv.
       intros y Hiny.
       unfold add_val at 1 3 4 5.
-      destruct (string_dec v y); subst; auto.
-      destruct (string_dec x y); subst; auto; [contradiction|].
+      destruct (var_dec v y); subst; auto.
+      destruct (var_dec x y); subst; auto; [contradiction|].
+      apply tm_rep_change_vv.
+      intros z Hinz. unfold add_val.
+      destruct (var_dec x z); subst; auto.
+      (*Here, get contradiction with bound*)
+      exfalso. apply (Hbnd z); auto.
+Qed.
 
-      erewrite tm_rep_change_vv.
-      2: { intros y1 Hiny1. apply add }
+Lemma fmla_subst_unsafe_rep (v: var) (t: tm) (f: fmla) :
+  (*Ensure no capture: no variable free in t can be bound in t1*)
+  (forall x, In x (tm_fv t) -> In x (fmla_bnd f) -> False) ->
+  forall (vv: val), fmla_rep vv (fmla_subst_unsafe v t f) <->
+  fmla_rep (add_val v (tm_rep vv t) vv) f.
+Proof.
+  induction f as [| | | f IH | [x f] IH | [x f] IH]; simpl; auto; intros Hbnd vv; try setoid_rewrite in_app_iff in Hbnd;
+  try solve[rewrite !tm_subst_unsafe_rep by eauto; reflexivity].
+  - apply binop_rep_congr; eauto.
+  - rewrite IH by eauto; reflexivity.
+  - destruct (var_dec v x); subst.
+    + setoid_rewrite fmla_rep_change_vv. reflexivity.
+      2: intros y Hiny; rewrite add_val_twice; reflexivity.
+      auto.
+    + setoid_rewrite IH; eauto.
+      simpl. setoid_rewrite fmla_rep_change_vv. reflexivity.
+      1: intros y Hiny; reflexivity.
+      intros y Hiny. unfold add_val at 1 2 3 5.
+      destruct (var_dec x y); subst; auto;
+      destruct (var_dec v y); subst; auto; try contradiction.
+      apply tm_rep_change_vv.
+      intros z Hinz. unfold add_val. destruct (var_dec x z); subst; auto. 
+      exfalso. apply (Hbnd z); auto.
+  - destruct (var_dec v x); subst.
+    + setoid_rewrite fmla_rep_change_vv. reflexivity.
+      2: intros y Hiny; rewrite add_val_twice; reflexivity.
+      auto.
+    + setoid_rewrite IH; eauto.
+      simpl. setoid_rewrite fmla_rep_change_vv. reflexivity.
+      1: intros y Hiny; reflexivity.
+      intros y Hiny. unfold add_val at 1 2 3 5.
+      destruct (var_dec x y); subst; auto;
+      destruct (var_dec v y); subst; auto; try contradiction.
+      apply tm_rep_change_vv.
+      intros z Hinz. unfold add_val. destruct (var_dec x z); subst; auto. 
+      exfalso. apply (Hbnd z); auto.
+Qed.
+
+(*Bindings and Variables*)
+
+(*Idea: we have counter - all bindings and counters can ONLY
+  be created through these functions*)
+Module ZVal <: BigIntVal.
+Definition val := CoqBigInt.zero.
+End ZVal.
+
+Module C := MakeCtr ZVal.
+
+Import MonadNotations.
+Local Open Scope state_scope.
+
+Definition create_var (name: string) : ctr var :=
+  _ <- C.incr tt ;;
+  i <- C.get tt ;;
+  st_ret (name, i).
+
+Definition rename_var (v: var) : ctr var :=
+  create_var (fst v).
+
+(*Idea: in OCaml, these are opaque - ONLY way to construct bindings*)
+Definition t_open_bound (b: tm_bound) : ctr (var * tm) :=
+  let (v, t) := b in
+  v1 <- rename_var v ;;
+  st_ret (v1, tm_subst_unsafe v (Tvar v1) t).
+
+Definition t_close_bound (v: var) (t: tm) : tm_bound :=
+  (v, t).
+
+Definition f_open_bound (b: fmla_bound) : ctr (var * fmla) :=
+  let (v, f) := b in
+  v1 <- rename_var v ;;
+  st_ret (v1, fmla_subst_unsafe v (Tvar v1) f).
+
+Definition f_close_bound (v: var) (f: fmla) : fmla_bound :=
+  (v, f).
+
+(* Type Safe API *)
+Definition t_const (z: CoqBigInt.t) : tm := Tconst z.
+Definition t_var (v: var) : tm := Tvar v.
+Definition t_add (tm1 tm2: tm) : tm := Top Add tm1 tm2.
+Definition t_mult (tm1 tm2: tm) : tm := Top Mult tm1 tm2.
+Definition t_let (t1: tm) (b: tm_bound) : tm := Tlet t1 b.
+Definition f_eq (tm1 tm2: tm) : fmla := Feq tm1 tm2.
+Definition f_lt (tm1 tm2: tm) : fmla := Flt tm1 tm2.
+Definition f_binop (b: binop) (f1 f2: fmla) : fmla := Fbinop b f1 f2.
+Definition f_not (f: fmla) : fmla := Fnot f.
+Definition f_forall (b: fmla_bound) : fmla := Fforall b.
+Definition f_exists (b: fmla_bound) : fmla := Fexists b.
+
+(*Because t_open_bound is no longer structurally recursive,
+  we need a [size] metric*)
+Fixpoint tm_size (t: tm) : nat :=
+  match t with
+  | Tconst _ => 1
+  | Tvar _ => 1
+  | Top _ t1 t2 => 1 + tm_size t1 + tm_size t2
+  | Tlet t1 (x, t2) => 1 + tm_size t1 + tm_size t2
+  end.
+
+(*Substituting a variable for a variable does not change size*)
+Lemma tm_subst_unsafe_var_size v1 v2 t:
+  tm_size (tm_subst_unsafe v1 (Tvar v2) t) = tm_size t.
+Proof.
+  induction t as [| | | t1 [x t2] IH1 IH2]; simpl; auto.
+  - destruct (var_dec _ _); reflexivity.
+  - rewrite IH1. destruct (var_dec v1 x); auto.
+Qed.  
+
+(*Binding-safe traversal*)
+From Equations Require Import Equations.
+Require Import Lia.
+(*Probably don't need but makes things much easier*)
+Require Import Coq.Logic.FunctionalExtensionality.
+Section SafeTraverse.
+Local Obligation Tactic := simpl; try lia.
+
+(* Lemma size_add1 t1 t2: (tm_size t1 < tm_size (Tadd t1 t2))%nat.
+Proof. simpl; lia. Qed.
+Lemma size_add2 t1 t2: (tm_size t2 < tm_size (Tadd t1 t2))%nat.
+Proof. simpl; lia. Qed.
+Lemma size_mult1 t1 t2: (tm_size t1 < tm_size (Tmult t1 t2))%nat.
+Proof. simpl; lia. Qed.
+Lemma size_mult2 t1 t2: (tm_size t2 < tm_size (Tmult t1 t2))%nat.
+Proof. simpl; lia. Qed. *)
+
+(*Express each case as function*)
+(*For OCaml purposes, NOT dependently typed (but it would be
+  easy to write an identical dependently typed version)*)
+Variable (T: Type).
+Variable (const_case: forall (c: Z), ctr T)
+  (var_case: forall (x: var), ctr T)
+  (op_case: forall (o: intop) (t1 t2: tm) (r1 r2: T), ctr T)
+  (mult_case: forall (t1 t2: tm) (r1 r2: T), ctr T)
+  (*NOTE: recursive case 2 on [t_open_bound] - b is the NEW variable*)
+  (let_case: forall (t1: tm) (x: var) (t2: tm) (r1 r2: T), ctr T).
+
+Equations tm_traverse (tm1: tm) : ctr T by wf (tm_size tm1) lt :=
+  tm_traverse (Tconst c) := const_case c;
+  tm_traverse (Tvar x) := var_case x;
+  tm_traverse (Top o t1 t2) :=
+    v1 <- tm_traverse t1 ;;
+    v2 <- tm_traverse t2 ;;
+    op_case o t1 t2 v1 v2;
+  tm_traverse (Tlet t1 b) :=
+    v1 <- tm_traverse t1 ;;
+    (*Need dependent types here to have enough information for the proof*)
+    st_bind_dep _ _ _ (t_open_bound b)
+      (fun y s Heq => 
+        v2 <- (tm_traverse (snd y)) ;;
+        let_case t1 (fst y) (snd b) v1 v2).
+Next Obligation.
+intros t1 [v1 t2] _ _ y s Hy; subst.
+simpl.
+rewrite tm_subst_unsafe_var_size. lia.
+Defined.
+Next Obligation.
+intros t1 b _; destruct b; simpl; lia.
+Defined.
+(* 
+Fixpoint tm_traverse' (tm1: tm) (ACC: Acc lt (tm_size tm1)) {struct ACC} : ctr T.
+Proof.
+  destruct tm1 as [c | v | t1 t2 | t1 t2 | t1 b].
+  - exact (const_case c).
+  - exact (var_case v).
+  - exact (r1 <- tm_traverse' t1 (Acc_inv ACC (size_add1 _ _)) ;;
+    r2 <- tm_traverse' t2 (Acc_inv ACC (size_add2 _ _));;
+    add_case t1 t2 r1 r2).
+  - exact (r1 <- tm_traverse' t1 (Acc_inv ACC (size_mult1 _ _)) ;;
+    r2 <- tm_traverse' t2 (Acc_inv ACC (size_mult2 _ _));;
+    mult_case t1 t2 r1 r2).
+  - refine (
+     v1 <- tm_traverse' t1 (Acc_inv ACC _) ;;
+    x <- t_open_bound b ;;
+    v2 <- tm_traverse' (snd x) (Acc_inv ACC _) ;;
+    let_case t1 (fst x) (snd b) v1 v2).
+    Show Proof. *)
+
+(*Now prove this equivalent to the non-dependent version*)
+(*Use funext*)
+Lemma tm_traverse_let (tm1: tm) (b: tm_bound) :
+  tm_traverse (Tlet tm1 b) =
+    v1 <- tm_traverse tm1 ;;
+    x <- t_open_bound b ;;
+    v2 <- tm_traverse (snd x) ;;
+    let_case tm1 (fst x) (snd b) v1 v2.
+Proof.
+  simp tm_traverse. f_equal.
+  apply functional_extensionality.
+  unfold st_bind, st_bind_dep, bind, Monad_state. simpl. intros x.
+  f_equal.
+  apply functional_extensionality; intros i.
+  destruct (runState (t_open_bound b)) eqn : Hr.
+  reflexivity.
+Qed.
+
+(*TODO: do we need an induction principle?*)
+End SafeTraverse.
+
+(*Safe substitution*)
+Definition sub_t  (v: var) (t: tm) (tm1: tm) : ctr tm :=
+  tm_traverse tm 
+    (fun c => st_ret (Tconst c))
+    (fun x => st_ret (if var_dec v x then t else (Tvar x)))
+    (fun o t1 t2 r1 r2 =>  st_ret (Top o r1 r2))
+    (fun t1 x t2 r1 r2 => st_ret (Tlet r1 (x, r2))) tm1.
+
+(*TODO: move*)
+
+(*From Hoare State Monad paper*)
+(*Instead of dependent types/Program, we have separate Prop*)
+(*TODO: not polymorphic enough*)
+Definition st_spec {A B: Type} (Pre: A -> Prop) (s: st A B)
+  (Post: A -> B -> A -> Prop) : Prop :=
+  forall i, Pre i -> Post i (fst (runState s i)) (snd (runState s i)).
+
+Lemma st_spec_ret {A B: Type} (x: B):
+  st_spec (fun _ => True) (st_ret x) (fun (s1: A) r s2 => s1 = s2 /\ r = x).
+Proof.
+  unfold st_spec; simpl; auto.
+Qed.
+
+Lemma st_spec_bind {St A B: Type} (P1 : St -> Prop) (P2: A -> St -> Prop) 
+  Q1 Q2 (a: st St A) (b: A -> st St B):
+  (st_spec P1 a Q1) ->
+  (forall x, st_spec (P2 x) (b x) (Q2 x)) ->
+  st_spec (fun s1 => P1 s1 /\ forall x s2, Q1 s1 x s2 -> P2 x s2)
+    (st_bind b a) 
+    (fun s1 y s3 => exists x s2, Q1 s1 x s2 /\ Q2 x s2 y s3).
+Proof.
+  unfold st_spec; simpl; intros Ha Hb i [Hi Himpl].
+  exists (fst (runState a i)). exists (snd (runState a i)).
+  split; auto.
+  destruct (runState a i) as [v s] eqn : Hrun; simpl.
+  apply Hb. apply Himpl. specialize (Ha _ Hi).
+  rewrite Hrun in Ha; apply Ha.
+Qed.
+
+(*A weakening lemma*)
+Lemma st_spec_weaken {A B: Type} (P1 P2: A -> Prop) (Q1 Q2: A -> B -> A -> Prop)
+  (s: st A B):
+  (forall i, P2 i -> P1 i) ->
+  (forall i x f, Q1 i x f -> Q2 i x f) ->
+  st_spec P1 s Q1 ->
+  st_spec P2 s Q2.
+Proof.
+  unfold st_spec; intros; auto.
+Qed.
+
+Lemma st_spec_weaken_pre {A B: Type} (P1 P2: A -> Prop) Q
+  (s: st A B):
+  (forall i, P2 i -> P1 i) ->
+  st_spec P1 s Q ->
+  st_spec P2 s Q.
+Proof.
+  intros Hp.
+  apply st_spec_weaken; auto.
+Qed.
+(*Much nicer for proofs*)
+(*NOTE: st_spec_ret too weak (unlike paper) - we do in fact want
+  to know that the precondition holds*)
+Lemma prove_st_spec_ret {A B: Type} (P1 : A -> Prop) (Q1: A -> B -> A -> Prop) 
+  (x: B):
+  (forall i, P1 i -> Q1 i x i) ->
+  st_spec P1 (st_ret x) Q1.
+Proof.
+  intros Hq.
+  unfold st_spec, st_ret. simpl. auto.
+Qed.
+
+(*TODO: names should be consistent*)
+
+Lemma prove_st_spec_bnd {St A B: Type} (P1 : St -> Prop) (P2: A -> St -> Prop) 
+  Q1 Q2 Q3 (a: st St A) (b: A -> st St B):
+  (*Hmm, what if Q1 does not use initial state?*)
+  (st_spec P1 a Q1) ->
+  (forall x, st_spec (P2 x) (b x) (Q2 x)) ->
+  (*Weaken head*)
+  (forall i, P1 i -> (forall x s2, Q1 i x s2 -> P2 x s2)) ->
+  (*Weaken rest*)
+  (forall s1 s2 s3 x y, Q1 s1 x s2 -> Q2 x s2 y s3 -> Q3 s1 y s3) ->
+  st_spec P1 (st_bind b a) Q3.
+Proof.
+  intros Ha Hb Hw1 Hw2. eapply st_spec_weaken.
+  3: apply st_spec_bind. all: eauto; simpl.
+  - intros i Hp. split; auto. apply Hw1. auto.
+  - intros i x f [y [s [Hq1 Hq2]]]; eapply Hw2; eauto.
+Qed.
+
+(*Version that does not depend on initial state (i.e. Q2 does not depend on x)*)
+(*If Q1 does not depend on initial state, then Q1 and P2 same*)
+(*And if Q2 does not depend on initial state, then Q2 and Q3 same*)
+Lemma prove_st_spec_bnd_nondep {St A B: Type} (P1 : St -> Prop)
+  Q1 Q2 Q3 a (b: A -> st St B):
+  (*Hmm, what if Q1 does not use initial state?*)
+  (st_spec P1 a (fun _ => Q1)) ->
+  (forall x, st_spec (Q1 x) (b x) (fun _ => (Q2 x))) ->
+  (*Weaken rest*)
+  (forall s2 s3 x y, Q1 x s2 -> Q2 x y s3 -> Q3 y s3) ->
+  st_spec P1 (st_bind b a) (fun _ => Q3).
+Proof.
+  intros Ha Hb Hw. eapply prove_st_spec_bnd; eauto.
+  apply Hb. simpl. auto.
+Qed.
+
+Lemma st_spec_and {A B: Type} (P1 P2: A -> Prop) Q1 Q2 (o: st A B):
+  st_spec P1 o Q1 ->
+  st_spec P2 o Q2 ->
+  st_spec (fun i => P1 i /\ P2 i) o (fun s1 r s2 => Q1 s1 r s2 /\ Q2 s1 r s2).
+Proof.
+  unfold st_spec. intros Hp1 Hp2 i [Hi1 Hi2]. auto.
+Qed.
+
+Lemma st_spec_get {A: Type} (P1: A -> Prop) (Q1: A -> A -> A -> Prop):
+  (forall i, P1 i -> Q1 i i i) ->
+  st_spec P1 (State.st_get) Q1.
+Proof.
+  intros Hpq. unfold st_spec; simpl. auto.
+Qed.
+
+Lemma st_spec_set {A: Type} (x: A) (P1: A -> Prop) (Q1: A -> unit -> A -> Prop):
+  (forall i, P1 i -> Q1 i tt x) ->
+  st_spec P1 (State.st_set x) Q1.
+Proof.
+  intros Hpq. unfold st_spec; simpl. auto.
+Qed.
+
+(*Prove dep bnd*)
+Lemma prove_st_spec_dep_bnd {St A B: Type} (P1 : St -> Prop) (P2: A -> St -> Prop) 
+  Q1 Q2 Q3 (a: st St A) (b: forall (b: A) (s: St), b = fst (runState a s) -> st St B):
+  (*Hmm, what if Q1 does not use initial state?*)
+  (st_spec P1 a Q1) ->
+  (forall x s Heq, st_spec (P2 x) (b x s Heq) (Q2 x)) ->
+  (*Weaken head*)
+  (forall i, P1 i -> (forall x s2, Q1 i x s2 -> P2 x s2)) ->
+  (*Weaken rest*)
+  (forall s1 s2 s3 x y, Q1 s1 x s2 -> Q2 x s2 y s3 -> Q3 s1 y s3) ->
+  st_spec P1 (st_bind_dep _ _ _ a b) Q3.
+Proof.
+  (*Very, very tricky due to dependent types*)
+  unfold st_spec; simpl. intros Ha Hb Hi Himpl i Hpi.
+  generalize dependent (@eq_refl _ (fst (runState a i))).
+  specialize (Hb (fst (runState a i)) i).
+  generalize dependent (b (fst (runState a i)) i).
+  intros b2 Hb2.
+  specialize (Ha i).
+  generalize dependent (runState a i).
+  intros. eapply Himpl; eauto.
+Qed.
+
+(*And simpler version*)
+Lemma prove_st_spec_dep_bnd_nondep {St A B: Type} (P1 : St -> Prop)
+  Q1 Q2 Q3 a (b: forall (b: A) (s: St), b = fst (runState a s) -> st St B):
+  (st_spec P1 a (fun _ => Q1)) ->
+  (forall x s Heq, st_spec (Q1 x) (b x s Heq) (fun _ => (Q2 x))) ->
+  (*Weaken rest*)
+  (forall s2 s3 x y, Q1 x s2 -> Q2 x y s3 -> Q3 y s3) ->
+  st_spec P1 (st_bind_dep _ _ _ a b) (fun _ => Q3).
+Proof.
+  intros Ha Hb Hw. eapply prove_st_spec_dep_bnd; eauto.
+  apply Hb. simpl. auto.
+Qed.
+
+(*Counter*)
+Lemma st_spec_incr (P1: CoqBigInt.t -> Prop) 
+  (Q1: CoqBigInt.t -> unit -> CoqBigInt.t -> Prop):
+  (forall i, P1 i -> Q1 i tt (CoqBigInt.succ i)) ->
+  st_spec P1 (C.incr tt) Q1.
+Proof.
+  intros Hsucc. unfold st_spec; simpl. auto.
+Qed.
+
+(*Any constant invariant is preserved*)
+Lemma st_spec_const {A B: Type} (x: st A B) (P1 P2: Prop):
+  (P1 -> P2) ->
+  st_spec (fun _ => P1) x (fun _ _ _ => P2).
+Proof.
+  unfold st_spec; auto.
+Qed.
+
+(* Lemma st_spec_frame {A B: Type} (P1 P2: A -> Prop) Q1 (o: st A B):
+  st_spec P1 o Q1 ->
+  (st_spec P2 o (fun _ _ i => P2 i)) -> (*This property is preserved*)
+  st_spec (fun i => P2 i /\ P1 i) o (fun s1 r s2 => P2 s2 /\ Q1 s1 r s2).
+Proof.
+  unfold st_spec. intros Ho Hpres. intros Hspec.
+  intros i [Hp2 Hp1]. *)
 
 
-      symmetry. erewrite tm_rep_change_vv.
-      2: { intros y Hy. apply add_val_switch. auto. }
-      change (fun y => add_val v (tm_rep vv t)
-        (add_val x (tm_rep vv (tm_subst_unsafe v t t1)) vv) y) with 
-        (add_val v (tm_rep vv t)
-        (add_val x (tm_rep vv (tm_subst_unsafe v t t1)) vv)).
-      rewrite <- (IH2 (add_val x (tm_rep vv (tm_subst_unsafe v t t1)) vv)).
-      rewrite <- IH2.
-      simpl.
+(*TODO: move*)
+(* Definition st_prop {A B: Type} (P: A -> B -> Prop) (x: B) (s: st A B) : Prop :=
+  forall a, P a x -> P (runState s a). *)
 
-      rewrite add_val_switch.
+(*P is an invariant relating the inputs and outputs with the states
+  P1 is a property that holds on the output, assuming the invariant
+  holds of the input*)
+(* Definition st_spec {A B: Type} (P: A -> B -> Prop)
+  (P1: B -> Prop) (x: B) (s: st A B) :=
+  forall a, P a x ->
+    P (snd (runState s a)) (fst (runState s a)) /\
+    P1 (fst (runState s a)). 
+
+Lemma st_spec_bind {A B: Type} (P: A -> B -> Prop)
+  (P1 P2: B -> Prop) (x: B) (f: B -> st A B) (y: st A B):
+  st_spec P P2 x y -> (*NOTE: don't need P1 here*)
+  ( st_spec P P1 x (f x)) ->
+  st_spec P P1 x (st_bind f y).
+Proof.
+Admitted. *)
+  (* unfold st_spec, st_bind; simpl; intros Hx Hb a Ha.
+  destruct (runState y a) as [v s] eqn : Hrun; simpl.
+  apply Hb. specialize (Hx _ Ha).
+  rewrite Hrun in Hx. simpl in Hx. apply Hx.
+Qed.  *)
+
+(*Term well-formed wrt state - all variables have smaller indices*)
+Definition tm_vars t := tm_fv t ++ tm_bnd t.
+Definition tm_st_wf (i: CoqBigInt.t) (t: tm) : Prop :=
+  forall v, In v (tm_vars t) -> snd v < i.
+
+(*Prove correctness of substitution*)
+
+(*Traversal well-formed*)
+
+Section TraverseWf.
+Variable (T: Type).
+
+Print tm_traverse.
+
+(*Any term remains well-formed after any other term is traversed
+  (i.e. the counter only increases)*)
+(* Lemma traverse_wf wconstr wvar wadd wmult wlet tm1 tm2:
+  st_spec (fun s1 => tm_st_wf s1 tm2)
+    (tm_traverse T wconstr wvar wadd wmult wlet tm1)
+    (fun _ _ s2 => tm_st_wf s2 tm2).
+Proof.
+  apply tm_traverse_elim.
+  - intros c. apply prove_ simpl. *)
+
+End TraverseWf.
+(*First, prove well-formed*)
+Section SubCorrect.
+Variable (v: var) (t: tm).
+Definition sub_rep (vv: val) (tm1 tm2: tm) :=
+  tm_rep vv tm1 = tm_rep (add_val v (tm_rep vv t) vv) tm2.
+(* 
+Lemma t_open_bound_spec (tm1: tm) (b: tm_bound):
+  st_spec (fun i => tm_st_wf i tm1) (t_open_bound b) 
+    (fun _ b2 s2 => tm_st_wf s2 tm1 /\ (*Still wf*)
+    ~ In (fst b2) (tm_vars tm1) /\ (*New var in term's vars*)
+    ~ In (fst b2) (tm_vars (snd b)) /\ (*New var not in old term*)
+    (*semantics are same except v is mapped to new var*)
+    forall vv, tm_rep vv (snd b2) = tm_rep (add_val v (vv (fst b2)) vv) (snd b)).
+Proof.
+  unfold t_open_bound.
+  destruct b as [v2 t2].
+  apply prove_st_spec_bnd_nondep with (Q1:=fun v1 s1 => 
+    tm_st_wf s1 tm1 /\
+    ~ 
+    )
+    (Q2:=fun _ _ s2 => tm_st_wf s2 tm1); auto.
+  - unfold rename_var, create_var.
+    (*Here, use counter info*)
+    apply prove_st_spec_bnd_nondep with (Q1:=fun _ s1 => tm_st_wf s1 tm1)
+      (Q2:=fun _ _ s2 => tm_st_wf s2 tm1); auto.
+    + apply st_spec_incr. 
+      (*The only interesting part: if wf, still wf with succ*)
+      intros i. unfold tm_st_wf.
+      (*TODO: add result: i < CoqBigInt.succ i*)
+      intros Hlt x Hinx. 
+      assert (Hsucc: forall x, x < CoqBigInt.succ x) by (unfold CoqBigInt.succ; lia).
+      specialize (Hsucc i). specialize (Hlt _ Hinx). lia.
+    + intros _. apply prove_st_spec_bnd_nondep with (Q1:=fun _ s1 => tm_st_wf s1 tm1)
+      (Q2:=fun _ _ s2 => tm_st_wf s2 tm1); auto.
+      * apply st_spec_get. auto.
+      * intros i. apply prove_st_spec_ret. auto.
+  - intros x. apply prove_st_spec_ret. auto.
+Qed.
+
+st_spec (fun i : CoqBigInt.t => tm_st_wf i t) (t_open_bound b)
+(fun (_ : CoqBigInt.t) (r : var * tm) (s2 : CoqBigInt.t) =>
+tm_st_wf s2 t /\ ~ In (fst r) (tm_fv t1)) *)
+
+Lemma t_open_bound_wf (tm1: tm) (b: tm_bound):
+  st_spec (fun i => tm_st_wf i tm1) (t_open_bound b) 
+    (fun _ _ s2 => tm_st_wf s2 tm1).
+Proof.
+  unfold t_open_bound.
+  destruct b as [v2 t2].
+  eapply prove_st_spec_bnd_nondep with (Q1:=fun _ s1 => tm_st_wf s1 tm1)
+    (Q2:=fun _ _ s2 => tm_st_wf s2 tm1); auto.
+  - unfold rename_var, create_var.
+    (*Here, use counter info*)
+    apply prove_st_spec_bnd_nondep with (Q1:=fun _ s1 => tm_st_wf s1 tm1)
+      (Q2:=fun _ _ s2 => tm_st_wf s2 tm1); auto.
+    + apply st_spec_incr. 
+      (*The only interesting part: if wf, still wf with succ*)
+      intros i. unfold tm_st_wf.
+      (*TODO: add result: i < CoqBigInt.succ i*)
+      intros Hlt x Hinx. 
+      assert (Hsucc: forall x, x < CoqBigInt.succ x) by (unfold CoqBigInt.succ; lia).
+      specialize (Hsucc i). specialize (Hlt _ Hinx). lia.
+    + intros _. apply prove_st_spec_bnd_nondep with (Q1:=fun _ s1 => tm_st_wf s1 tm1)
+      (Q2:=fun _ _ s2 => tm_st_wf s2 tm1); auto.
+      * apply st_spec_get. auto.
+      * intros i. apply prove_st_spec_ret. auto.
+  - intros x. apply prove_st_spec_ret. auto.
+Qed.
+
+Lemma sub_t_wf (tm2: tm) (tm1: tm):
+  st_spec (fun i => tm_st_wf i tm2)
+    (sub_t v t tm1)
+    (fun _ _ s2 => tm_st_wf s2 tm2). 
+Proof.
+  unfold sub_t.
+  apply tm_traverse_elim.
+  - intros c. apply prove_st_spec_ret. auto.
+  - intros x. apply prove_st_spec_ret. auto.
+  - intros o t1 t2 IH1 IH2.
+    apply prove_st_spec_bnd_nondep with (Q1:=fun r1 s1 => tm_st_wf s1 tm2)
+    (Q2:= fun _ t3 s4 => tm_st_wf s4 tm2); auto.
+    intros r1.
+    apply prove_st_spec_bnd_nondep with (Q1:=fun r2 s2 => tm_st_wf s2 tm2)
+    (Q2 := fun _ t3 s4 => tm_st_wf s4 tm2); auto.
+    intros r2. apply prove_st_spec_ret. auto.
+  - (*let case*) intros t1 b IH1 IH2.
+    (*eliminate dependent bind*)
+    (* rewrite <- (tm_traverse_equation_5 tm _ _ _ _
+      (fun _ x _ r1 r2 => st_ret (Tlet r1 (x, r2)))),
+    tm_traverse_let. *)
+    (*Now go through binds*)
+    apply prove_st_spec_bnd_nondep with (Q1:=fun r1 s1 => tm_st_wf s1 tm2)
+    (Q2:= fun _ t3 s4 => tm_st_wf s4 tm2); auto.
+    intros r1.
+    (*Here, need to reason about [t_open_bound]*)
+    (*TODO: is this right Q1 and Q2?*)
+    apply prove_st_spec_dep_bnd_nondep with (Q1:=fun v1 s1 => tm_st_wf s1 tm2)
+    (Q2:= fun _ t3 s4 => tm_st_wf s4 tm2); auto.
+    + apply t_open_bound_wf.
+    + (*Now use 2nd IH*)
+      intros b1 s1 Hb1.
+      apply prove_st_spec_bnd_nondep with (Q1:=fun v1 s1 => tm_st_wf s1 tm2)
+      (Q2:= fun _ t3 s4 => tm_st_wf s4 tm2); auto.
+      * (*Why we needed "dep" case - for IH premise*) eapply IH1; eauto.
+      * intros t2. apply prove_st_spec_ret. auto.
+Qed.
+
+Lemma tm_st_wf_op i o t1 t2:
+  tm_st_wf i t1 ->
+  tm_st_wf i t2 ->
+  tm_st_wf i (Top o t1 t2).
+Proof.
+Admitted.
+  (* unfold tm_st_wf. simpl. setoid_rewrite in_app_iff. 
+  intros H1 H2 x [Hinv | Hinv]; auto.
+Qed. *)
+
+Ltac destruct_all :=
+  repeat match goal with
+  | H: ?P /\ ?Q |-_ => destruct H
+  end.
+
+Ltac split_all :=
+  repeat match goal with
+  | |- ?P /\ ?Q => split
+  end.
+
+Ltac destruct_or :=
+  repeat match goal with
+  | H: ?P \/ ?Q |- _ => destruct H
+  end.
+
+Lemma tm_st_wf_op_iff i o t1 t2:
+  tm_st_wf i (Top o t1 t2) <->
+  tm_st_wf i t1 /\
+  tm_st_wf i t2.
+Proof.
+  unfold tm_st_wf, tm_vars; simpl.
+  repeat (setoid_rewrite in_app_iff). split; intros Hall; destruct_all;
+  split_all; intros; auto; destruct_or; auto.
+Qed.
+
+
+(* Lemma tm_st_wf_op_inv i o t1 t2: *)
+  (* tm_st_wf i (Top o t1 t2) ->
+  tm_st_wf i t1 /\
+  tm_st_wf i t2.
+Proof.
+  unfold tm_st_wf, tm_vars; simpl.
+  repeat (setoid_rewrite in_app_iff). intros Hall.
+  split; intros x [Hinv | Hinv]; auto.
+Qed. *)
+
+Lemma sub_rep_op o vv t1 t2 r1 r2:
+  sub_rep vv r1 t1 ->
+  sub_rep vv r2 t2 ->
+  sub_rep vv (Top o r1 r2) (Top o t1 t2).
+Proof.
+  unfold sub_rep. simpl. intros; f_equal; auto.
+Qed.
+
+
+
+Definition var_st_wf (i: CoqBigInt.t) (v: var) : Prop :=
+  snd v < i.
+
+Lemma sub_t_correct (tm1: tm) :
+  st_spec 
+    (fun i => tm_st_wf i t /\ tm_st_wf i tm1 /\ var_st_wf i v) 
+    (sub_t v t tm1)
+    (fun _ t2 i => tm_st_wf i t /\ tm_st_wf i tm1 /\ 
+      tm_st_wf i t2 /\ var_st_wf i v /\ forall vv, sub_rep vv t2 tm1).
+Proof.
+  unfold sub_t.
+  apply tm_traverse_elim.
+  - unfold sub_rep. intros c. simpl. apply prove_st_spec_ret.
+    intros i Hwf. simpl. destruct_all; split_all; auto.
+  - intros x. unfold sub_rep. simpl. apply prove_st_spec_ret.
+    intros i [Hwf1 [Hwf2 Hwfv]]. unfold add_val.
+    split_all; auto; destruct (var_dec v x); auto.
+  - intros o t1 t2 IH2 IH1.
+    (*First, change to t1 and t2 wf*)
+    apply st_spec_weaken with (P1:= fun i =>
+      tm_st_wf i t2 /\ (tm_st_wf i t /\ tm_st_wf i t1 /\ var_st_wf i v))
+    (Q1:=fun _ tm2 i =>
+      tm_st_wf i t /\ tm_st_wf i t1 /\ tm_st_wf i t2 /\ 
+      tm_st_wf i tm2 /\ var_st_wf i v /\ (forall vv, sub_rep vv tm2 (Top o t1 t2)));
+    try solve[intros; rewrite tm_st_wf_op_iff in *; intros; destruct_all; split_all; auto].
+    (*Now go through first IH*)
+    (*A bit tricky: we will need to separate out some preconditions
+      and prove they are preserved separately*)
+    apply prove_st_spec_bnd_nondep with (Q1:=fun r1 s1 =>
+      (*Stuff to prove separately*)
+      (tm_st_wf s1 t2) /\
+      (*Conclusions of IH1*)
+      (tm_st_wf s1 t /\
+      tm_st_wf s1 t1 /\
+      tm_st_wf s1 r1 /\
+      var_st_wf s1 v /\
+      (forall vv, sub_rep vv r1 t1)))
+    (*TODO: isn't this the same as post*)
+    (Q2:= fun _ t3 s4 =>
+      tm_st_wf s4 t /\
+      tm_st_wf s4 t1 /\
+      tm_st_wf s4 t2 /\
+      tm_st_wf s4 t3 /\
+      var_st_wf s4 v /\
+      (forall vv, sub_rep vv t3 (Top o t1 t2))); auto;
+    [apply st_spec_and; [apply sub_t_wf |apply IH1] |].
+    (*Now do same for t2 part*)
+    intros r1.
+    (*Again weaken to get hyps in right place*)
+    apply st_spec_weaken_pre with (P1:= fun i =>
+      (*Not needed in IH*)
+      (tm_st_wf i t1 /\ tm_st_wf i r1 /\ (forall vv : val, sub_rep vv r1 t1)) /\ 
+      (*In IH*)
+      (tm_st_wf i t /\ tm_st_wf i t2 /\ var_st_wf i v));
+    [intros; destruct_all; split_all; auto|].
+    apply prove_st_spec_bnd_nondep with (Q1:=fun r2 s2 =>
+      (*Suff to prove separately*)
+      (tm_st_wf s2 t1 /\ tm_st_wf s2 r1 /\ (forall vv : val, sub_rep vv r1 t1)) /\
+      (*Concludions of IH2*)
+      (tm_st_wf s2 t /\ tm_st_wf s2 t2 /\ tm_st_wf s2 r2 /\ var_st_wf s2 v /\
+        (forall vv, sub_rep vv r2 t2)))
+    (Q2:=fun _ t3 s4 =>
+      tm_st_wf s4 t /\ tm_st_wf s4 t1 /\ tm_st_wf s4 t2 /\
+      tm_st_wf s4 t3 /\ var_st_wf s4 v /\
+      (forall vv, sub_rep vv t3 (Top o t1 t2))); auto;
+    [apply st_spec_and; [| apply IH2; auto]|].
+    1: { 
+      apply st_spec_and; [apply sub_t_wf| apply st_spec_and];
+      [apply sub_t_wf | apply st_spec_const]; auto.
+    }
+    (*Now at end, prove goal*)
+    intros r2.
+    apply prove_st_spec_ret.
+    intros i [[Hwf1 [Hwfr1 Hval1]] [Hwft [Hwf2 [Hwfr2 [Hwfv Hval2]]]]].
+    split_all; auto.
+    + rewrite tm_st_wf_op_iff. split; auto.
+    + intros vv. apply sub_rep_op; auto.
+  - (*Tlet - interesting case*)
+    intros t1 b1 IHt1 IHb.
+    (*TODO: prove iff lemma for tm_st_wf Tlet*)
+    (*idea: first only consumes t1, gives v1
+      then in [t_open_bound], get that
+      1. new var is not in bound *)
+      Print unsafe_s.
+
+
+    1: {  }
+
+    (Q1:=fun _ tm2 i =>
+      tm_st_wf i t /\ tm_st_wf i t1 /\ tm_st_wf i t2 /\ 
+      tm_st_wf i tm2 /\ var_st_wf i v /\ (forall vv, sub_rep vv tm2 (Top o t1 t2)));
+
+    + (*Prove t1 part*)
+      .
+
+  (*Idea: P2: after we have IH1, Q2, have full result (rest)*)
+    apply prove_st_spec_bnd_nondep with (Q1:=fun r1 s1 =>
+      (tm_st_wf s1 t /\ 
+      tm_st_wf s1 t2) /\
+      tm_st_wf s1 t1 /\
+      tm_st_wf s1 r1 /\
+      (forall vv, sub_rep vv r1 t1))
+    (Q2:= fun _ t3 s4 =>
+      tm_st_wf s4 t /\
+      tm_st_wf s4 (Top o t1 t2) /\
+      tm_st_wf s4 t3 /\
+      (forall vv, sub_rep vv t3 (Top o t1 t2))); auto.
+    1: { eapply st_spec_weaken. 3: apply IH2. all: simpl; auto.
+      intros; destruct_all; auto.
+      intros; destruct_all; auto. }
+    intros r1.
+    (*Idea: prove stronger Post (post of IH)
+      combine with "and"*)
+    apply prove_st_spec_bnd_nondep with
+    (Q1:= fun r2 s2 =>
+      (tm_st_wf s2 t /\
+      tm_st_wf s2 t2 /\
+      tm_st_wf s2 r2 /\
+      (forall vv, sub_rep vv r2 t2)) /\
+      (
+      tm_st_wf s2 t1 /\
+      tm_st_wf s2 r1 /\
+      (forall vv, sub_rep vv r1 t1))
+      )
+    (Q2:= fun _ t3 s4 =>
+      tm_st_wf s4 t /\
+      tm_st_wf s4 (Top o t1 t2) /\
+      tm_st_wf s4 t3 /\
+      (forall vv, sub_rep vv t3 (Top o t1 t2))); auto.
+    +  (*Need to use "and" lemma to split*)
+      (*Forst, get t and t2 together*)
+      apply st_spec_and. [apply IH1; auto|].
+      (*Now, need to show that [tm_st_wf] and [sub_rep] are preserved*)
+      (*Separate lemma to show just wf preservation*)
+      apply st_spec_and; [apply sub_t_wf|].
+      apply st_spec_const. auto.
+    + intros r2. apply prove_st_spec_ret.
+      intros i [[Hwft [Hwfr2 Hrep2]] [Hwfr1 Hrep1]].
+      split; [|split]; auto.
+      (*Prove props preserved by [Top]*)
+      -- apply tm_st_wf_op; auto.
+      -- intros vv. apply sub_rep_op; auto.
+  - (*let case - interesting*)
+    intros t1 b IHb IHt1.
+    (*First, use IHt1*)
+    apply prove_st_spec_bnd_nondep with (Q1:=fun r1 s1 =>
+      tm_st_wf s1 t /\ 
+      tm_st_wf s1 r1 /\
+      (forall vv, sub_rep vv r1 t1))
+    (Q2:= fun _ t3 s4 =>
+      tm_st_wf s4 t /\
+      tm_st_wf s4 t3 /\
+      (forall vv, sub_rep vv t3 (Tlet t1 b))); auto.
+    intros r1.
+    (*Now open the bound - need to know that new var not in freevars of t*)
+    apply prove_st_spec_dep_bnd_nondep with 
+    (Q1:=fun y1 s2 => 
+      tm_st_wf s2 t /\ 
+      tm_st_wf s2 r1 /\
+      (forall vv, sub_rep vv r1 t1) /\
+      ~ In (fst y1) (tm_fv t1)) (*TODO: see if this is enough*)
+     (Q2:= fun _ t3 s4 =>
+      tm_st_wf s4 t /\
+      tm_st_wf s4 t3 /\
+      (forall vv, sub_rep vv t3 (Tlet t1 b))); auto.
+    + (*Prove [t_open_bound] part*)
+      (*Want to get rid of r1 parts, not interesting*)
+      eapply st_spec_weaken with (P1:= fun i =>
+        (tm_st_wf i r1 /\ (forall vv : val, sub_rep vv r1 t1)) /\
+        tm_st_wf i t) (Q1 := fun _ x f =>
+        (tm_st_wf f r1 /\ (forall vv : val, sub_rep vv r1 t1)) /\
+        (tm_st_wf f t /\ ~ In (fst x) (tm_fv t1))); auto.
+      1: { intros i. intros [Hwf1 [Hwf2 Hvv]]. auto. }
+      1: { intros _ x f [[Hwf1 Hvv] [Hwf2 Hfv]]; auto. }
+      (*separate out interesting parts*)
+      apply st_spec_and.
+      1: { apply st_spec_and; [apply t_open_bound_wf|apply st_spec_const]; auto. }
+      (*Prove postcondition of [t_open_bound]*)
+      {
+        unfold t_open_bound.
+        destruct b as [v2 t2]. 
+        eapply prove_st_spec_bnd_nondep with (Q1:= fun v1 s1 => tm_st_wf s1 t /\
+        ~ In v1 (tm_fv t1)) (Q2:=fun _ r s2 =>
+          tm_st_wf s2 t /\ ~ In (fst r) (tm_fv t1)); auto.
+        - (*[rename_var] goal*)
+          unfold rename_var.
+
+      }
+        *
+
+
+eapply prove_st_spec_bnd_nondep with (Q1:=fun _ s1 => tm_st_wf s1 tm1)
+    (Q2:=fun _ _ s2 => tm_st_wf s2 tm1); auto.
+  - unfold rename_var, create_var.
+    (*Here, use counter info*)
+    apply prove_st_spec_bnd_nondep with (Q1:=fun _ s1 => tm_st_wf s1 tm1)
+      (Q2:=fun _ _ s2 => tm_st_wf s2 tm1); auto.
+    + apply st_spec_incr. 
+      (*The only interesting part: if wf, still wf with succ*)
+      intros i. unfold tm_st_wf.
+      (*TODO: add result: i < CoqBigInt.succ i*)
+      intros Hlt x Hinx. 
+      assert (Hsucc: forall x, x < CoqBigInt.succ x) by (unfold CoqBigInt.succ; lia).
+      specialize (Hsucc i). specialize (Hlt _ Hinx). lia.
+    + intros _. apply prove_st_spec_bnd_nondep with (Q1:=fun _ s1 => tm_st_wf s1 tm1)
+      (Q2:=fun _ _ s2 => tm_st_wf s2 tm1); auto.
+      * apply st_spec_get. auto.
+      * intros i. apply prove_st_spec_ret. auto.
+  - intros x. apply prove_st_spec_ret. auto.
+
+
+      * apply 
+      1: { intros i.
+      
+      
+       rewrite and_comm. }
+      apply st_spec_and; [apply t_open_bound_wf|].
+      apply st_spec_and; [apply t_open_bound_wf|].
+       Search t_open_bound.
     
-     rewrite IH2. apply tm_rep_change_vv. intros y Hy.
-      rewrite add_val_twice.
-      rewrite add_val_switch.
-      unfold add_val. destruct (string_dec v y); subst; auto.
-      destruct (string_dec x y); subst; auto.
-      * apply tm_rep_change_vv.
+    tm_st_wf s1 tm2)
+    (Q2:= fun _ t3 s4 => tm_st_wf s4 tm2); auto.
+
+
+    * auto.
+    + auto.
+  - 
+          unfold tm_st_wf.
+        
+         [Hwft [Hwfr2 [Hrep2 [Hwfr1 Hrep1]]]].
+
+        
+
+(* eapply st_spec_weaken with (Q1:=
+        (fun _ t3 s4 =>
+          (tm_st_wf )
+        
+        ).
+      3: { apply st_spec_and.  }
+      (*Idea: in precondition, add " /\ True"
+        then prove "and" *)
+      eapply st_spec_weaken.
+      3: {
+        apply st_spec_and. apply IH1.
+      }
+      apply st_spec_and.
+      * apply IH1.*)
+      *
+      (Q2 := fun _ t3 t4 =>
+        ).
+      1: eapply st_spec_weaken; [| | apply IH1; auto].
+      1: apply IH1.
+       (Q1:=fun r2 s2 =>
+      tm_st_wf s2 t /\
+      tm_st_wf s2 r1 /\
+      (forall vv, sub_rep vv r1 t1) /\
+      tm_st_wf s2 r2 /\
+      (forall vv, sub_rep vv r2 t2)).
+      * eapply st_spec_weaken. 3: apply IH1. 
+        -- intros i [Hi _]; exact Hi.
+        -- simpl. intros _  apply IH1.
+      
+       with 
+      (*Q1: after IH2*)
+      (Q1:= fun _ r2 s2 =>
+      tm_st_wf s2 t /\
+      tm_st_wf s2 r1 /\
+      (forall vv, sub_rep vv r1 t1) /\
+      tm_st_wf s2 r2 /\
+      (forall vv, sub_rep vv r2 t2))
+      (*P2, almost the same - *)
+      (P2 := fun r2 s2 =>
+      tm_st_wf s2 t /\
+      tm_st_wf s2 r1 /\
+      (forall vv, sub_rep vv r1 t1) /\
+      tm_st_wf s2 r2 /\
+      (forall vv, sub_rep vv r2 t2)).
+      
+      (Q2:= fun _ _ t3 s4 =>
+        tm_st_wf s4 t /\
+        tm_st_wf s4 t3 /\
+        (forall vv, sub_rep vv t3 (Tadd t1 t2))).
+      * apply st_spec_weaken with
+        (Q1:= fun s2 ). 3: apply IH1; auto.
+        -- simpl. intros i [H1 _]; auto.
+        -- 
+      
+       apply prove_st_spec_ret.
+    
+     eapply prove_st_spec_bnd with 
+      (P2:= fun tm i => tm_st_wf i t /\ 
+        (forall vv, sub_rep vv x t1) /\ (forall vv, sub_rep vv tm t2))
+      (Q1:= fun s1 tm s2 => 
+        tm_st_wf s2 t /\
+        tm_st_wf s2 tm /\
+        (forall vv, sub_rep vv x t1) /\ (forall vv, sub_rep vv tm t2)).
+      * eapply st_spec_weaken.
+        1: { intros i [Hw H2]. apply Hw. }
+        2: apply IH1; auto.
+        intros s1 x1 s2. simpl. intros [Hwf1 [Hwf2 Hval1]].
+         
+       3: apply IH1; auto. all: simpl; auto.
+        -- intros i [Hi H2]; auto.
+        --  
+    (Q1:=(fun (s1 : CoqBigInt.t) (t2 : tm) (s2 : CoqBigInt.t) =>
+tm_st_wf s1 t /\
+tm_st_wf s2 t2 /\ (forall vv : val, tm_rep vv t2 =
+tm_rep (add_val v (tm_rep vv t) vv) t1)))
+(Q2:=(fun (v2 : tm)(s2: CoqBigInt.t)(t3: tm) (s3: CoqBigInt.t) =>
+  tm_st_wf s2 v2 /\
+  tm_st_wf s3 t3 /\
+  (forall vv, tm_rep vv t3 = tm_rep (add_val v (tm_rep vv t) vv) t3))).
+  + apply IH2.
+  + intros x. apply prove_st_spec_bnd with (P2:= fun tm i => tm_st_wf i t)
+      (Q1:= (fun (s1 : CoqBigInt.t) (t3 : tm) (s2 : CoqBigInt.t) =>
+tm_st_wf s1 t /\
+tm_st_wf s2 t3 /\ (forall vv : val, tm_rep vv t3 =
+tm_rep (add_val v (tm_rep vv t) vv) t2)))
+(Q2:=(fun (v2 : tm)(s2: CoqBigInt.t)(t3: tm) (s3: CoqBigInt.t) =>
+  tm_st_wf s2 v2 /\
+  tm_st_wf s3 t3 /\
+  (forall vv, tm_rep vv t3 = tm_rep (add_val v (tm_rep vv t) vv) t3))).
+    * apply IH1; auto.
+    * intros y. apply prove_st_spec_ret. simpl. 
   
-   apply IH2.
+
+
+(fun (s1 : CoqBigInt.t) (t2 : tm) (s2 : CoqBigInt.t) =>
+  tm_st_wf s1 t /\
+  tm_st_wf s2 t2 /\ (forall vv : val, tm_rep vv t2 =
+  tm_rep (add_val v (tm_rep vv t) vv) t1))).
+(*     
+    
+     (P2:=fun tm i =>
+      tm_st_wf i t /\ tm_st_wf i tm /\
+      forall vv, tm_rep vv tm = tm_rep (add_val v (tm_rep vv t) vv) t1). *)
+    + apply IH2.
+    + intros x. apply prove_st_spec_bnd with (P2:= fun tm i => tm_st_wf i t)
+      (Q1:= (fun (s1 : CoqBigInt.t) (t3 : tm) (s2 : CoqBigInt.t) =>
+tm_st_wf s1 t /\
+tm_st_wf s2 t3 /\ (forall vv : val, tm_rep vv t3 =
+tm_rep (add_val v (tm_rep vv t) vv) t2)))
+(Q2:=()).
+      * apply IH1; auto.
+      * intros y. apply prove_st_spec_ret.
+
+
+       simpl. 
+      2: {}
+     apply prove_st_spec_ret.
+
+  
+    + intros vv. unfold 
+     simpl.
+     split_all.
+
+  
+   eapply st_spec_weaken. 3: apply st_spec_ret.
+    + simpl. auto.
+    + simpl. intros i x f [Hif Hx]; subst. auto.
+    all: auto.
+  unfold sub_t.
+
+
+  st_spec (fun i t1 => 
+    tm_st_wf i t /\ tm_st_wf i t1) (fun (tm2: tm) => 
+    forall vv, tm_rep vv tm2 = tm_rep (add_val v (tm_rep vv t) vv) tm1)
+  tm1 (sub_t v t tm1).
+Proof.
+  unfold sub_t.
+  apply tm_traverse_elim.
+  - intros c. simpl. unfold st_spec, tm_st_wf; simpl; intros; auto.
+  - intros x. simpl. unfold st_spec, tm_st_wf; simpl. intros i [Ht _]. 
+    split; [split|]; auto.
+    + intros y. (*we need to know that t does not introduce larger vars*) 
+      destruct (var_dec v x); simpl; auto. contradiction.
+    + intros vv. unfold add_val. destruct (var_dec v x); subst; simpl; auto.
+  - intros t1 t2 IH1 IH2.
+    eapply st_spec_bind.
+    2: {
+      eapply st_spec_bind.
+      2: {
+
+      } 
+    }
+    + apply IH2.
+     with (P2 := fun _ => True).
+    + 
+
   
   
-   f_equal; auto. 
-    + unfold add_val. destruct (string_dec v v); auto. contradiction.
-    + unfold add_val.
+   unfold st_spec in *; simpl in *. 
+
+
+
+      * unfold add_val. destruct (var_dec v v); auto. contradiction.
+      * unfold add_val. 
+   st_spec. simpl.
+
+    )
+  st_prop tm_st_wf tm1 ()
+
+  
+
+  (const_case: forall (c: Z), ctr T)
+  (var_case: forall (x: var), ctr T)
+  (add_case: forall (t1 t2: tm) (r1 r2: T), ctr T)
+  (mult_case: forall (t1 t2: tm) (r1 r2: T), ctr T)
+  (*NOTE: recursive case 2 on [t_open_bound]*)
+  (let_case: forall (t1: tm) (b: tm_bound) (r1 r2: T), ctr T).
+  
+   simpl.
+   intros x.
+  
+  
+   apply functional_extensionality. simpl.
+  
+   simpl.
+  f_equal.
+
+Lemma tm_traverse_eq (tm1: tm):
+  tm_traverse tm1 =
+  match tm1 with
+  | Tconst c => const_case c
+  | Tvar x => var_case x
+  | Tadd t1 t2 =>
+    v1 <- tm_traverse t1 ;;
+    v2 <- tm_traverse t2 ;;
+    add_case t1 t2 v1 v2
+  | Tmult t1 t2 =>
+    v1 <- tm_traverse t1 ;;
+    v2 <- tm_traverse t2 ;;
+    mult_case t1 t2 v1 v2
+  | Tlet 
+
+
+Equations tm_traverse (tm1: tm) : ctr T by wf (tm_size tm1) lt :=
+  tm_traverse (Tconst c) := const_case c;
+  tm_traverse (Tvar x) := var_case x;
+  tm_traverse (Tadd t1 t2) :=
+    v1 <- tm_traverse t1 ;;
+    v2 <- tm_traverse t2 ;;
+    add_case t1 t2 v1 v2;
+  tm_traverse (Tmult t1 t2) :=
+    v1 <- tm_traverse t1 ;;
+    v2 <- tm_traverse t2 ;;
+    mult_case t1 t2 v1 v2;
+  tm_traverse (Tlet t1 b) :=
+    v1 <- tm_traverse t1 ;;
+    (*Need dependent types here to have enough information for the proof*)
+    st_bind_dep _ _ _ (t_open_bound b)
+      (fun y s Heq => 
+        v2 <- (tm_traverse (snd y)) ;;
+        let_case t1 b v1 v2).
+
+
+  .
+
+
+(*Safe substitution*)
+From Equations Require Import Equations.
+Require Import Lia.
+Section SafeSub.
+Variable (v: var) (t: tm).
+
+(*Use Equations for now*)
+Obligation Tactic := simpl; try lia.
+Equations sub_t (tm1: tm) : ctr tm by wf (tm_size tm1) lt :=
+  sub_t (Tconst c) := st_ret (Tconst c);
+  sub_t (Tvar x) := st_ret (if var_dec x v then t else (Tvar x));
+  sub_t (Tadd t1 t2) :=
+    t1' <- sub_t t1 ;;
+    t2' <- sub_t t2 ;;
+    st_ret (Tadd t1' t2');
+  sub_t (Tmult t1 t2) :=
+    t1' <- sub_t t1 ;;
+    t2' <- sub_t t2 ;;
+    st_ret (Tmult t1' t2');
+  sub_t (Tlet t1 b) :=
+    t1' <- sub_t t1 ;;
+   (*Need dependent types here to have enough information for the proof*)
+    st_bind_dep _ _ _ (t_open_bound b)
+      (fun y s Heq => sub_t (snd y)).
+Next Obligation.
+intros t1 [v1 t2] _ _ y s Hy; subst.
+simpl.
+rewrite tm_subst_unsafe_var_size. lia.
+Defined.
+Next Obligation.
+intros t1 b _; destruct b; simpl; lia.
+Defined.
+
+End SafeSub.
+
+From Coq Require Import Extraction.
+
+Extraction sub_t.
+
+(*Subst*)
+
+unfold t_open_bound. simpl.
+
+intros; subst. 
+simpl.
+intros t1 b IH t2 bound v2. simpl in *.
+
+
+
+(*Use "Well Founded Recursion Done Right"*)
+Lemma size_add1 t1 t2: (tm_size t1 < tm_size (Tadd t1 t2))%nat.
+Proof. simpl; lia. Qed.
+Lemma size_add2 t1 t2: (tm_size t2 < tm_size (Tadd t1 t2))%nat.
+Proof. simpl; lia. Qed.
+Lemma size_mult1 t1 t2: (tm_size t1 < tm_size (Tmult t1 t2))%nat.
+Proof. simpl; lia. Qed.
+Lemma size_mult2 t1 t2: (tm_size t2 < tm_size (Tmult t1 t2))%nat.
+Proof. simpl; lia. Qed.
+Check st_bind_dep.
+Fixpoint sub_t (tm1: tm) (ACC: Acc lt (tm_size tm1)) : ctr tm :=
+  match tm1 return Acc lt (tm_size tm1) -> ctr tm with
+  | Tconst c => fun _ => st_ret (Tconst c)
+  | Tvar x => fun _ => st_ret (if var_dec x v then t else (Tvar x))
+  | Tadd t1 t2 => fun ACC => 
+    t1' <- sub_t t1 (Acc_inv ACC (size_add1 _ _)) ;;
+    t2' <- sub_t t2 (Acc_inv ACC (size_add2 _ _)) ;;
+    st_ret (Tadd t1' t2')
+  | Tmult t1 t2 => fun ACC =>
+    t1' <- sub_t t1 (Acc_inv ACC (size_mult1 _ _)) ;;
+    t2' <- sub_t t2 (Acc_inv ACC (size_mult2 _ _)) ;;
+    st_ret (Tmult t1' t2')
+  | Tlet t1 b => fun ACC =>
+    t1' <- sub_t t1 (Acc_inv ACC _) ;;
+    (*Need dependent types here to have enough information for the proof*)
+    st_bind_dep _ _ _ (t_open_bound b)
+      (fun y s Heq => sub_t (snd y) (Acc_inv ACC _))
+  end ACC.
+    
+     (sub_t (snd ))
+    y <-- s <-- Heq <-- (t_open_bound b) ;;
+    sub_t (snd y) (Acc_inv ACC _)
+  end ACC.
+
+
+Obligation Tactic := simpl; try lia.
+Equations sub_t (tm1: tm) : ctr tm by wf (tm_size tm1) lt :=
+  sub_t (Tconst c) := st_ret (Tconst c);
+  sub_t (Tvar x) := st_ret (if var_dec x v then t else (Tvar x));
+  sub_t (Tadd t1 t2) :=
+    t1' <- sub_t t1 ;;
+    t2' <- sub_t t2 ;;
+    st_ret (Tadd t1' t2');
+  sub_t (Tmult t1 t2) :=
+    t1' <- sub_t t1 ;;
+    t2' <- sub_t t2 ;;
+    st_ret (Tmult t1' t2');
+  sub_t (Tlet t1 b) :=
+    t1' <- sub_t t1 ;;
+    y <- t_open_bound b ;;
+    sub_t (snd y).
+Next Obligation.
+intros t1 b IH t2 bound v2. simpl in *.
+
+Fixpoint int_rect_aux (z: CoqBigInt.t) 
+  (ACC: Acc lt (Z.to_nat z)) {struct ACC} : P z :=
+  match CoqBigInt.lt z CoqBigInt.zero as b return
+  CoqBigInt.lt z CoqBigInt.zero = b -> P z with
+  | true => fun Hlt => neg_case _ Hlt
+  | false => fun Hlt =>
+    match CoqBigInt.eqb z CoqBigInt.zero as b return
+      CoqBigInt.eqb z CoqBigInt.zero = b -> P z with
+    | true => fun Heq => eq_rect _ P zero_case _ (eq_sym (zero_lemma _ Heq))
+    | false => fun Hneq => 
+      ind_case _ Hneq Hlt (int_rect_aux (CoqBigInt.pred z) 
+        (Acc_inv ACC (int_wf_lemma _ Hneq Hlt)))
+    end eq_refl
+  end eq_refl.
+
+  match tm1 with
+  | Tconst c => st_ret tm1
+  | Tvar x => st_ret (if var_dec x v then t else tm1)
+  | Tadd t1 t2 => 
+    t1' <- sub_t v t t1 ;;
+    t2' <- sub_t v t t2 ;;
+    st_ret (Tadd t1' t2')
+  | Tmult t1 t2 =>
+    t1' <- sub_t v t t1 ;;
+    t2' <- sub_t v t t2 ;;
+    st_ret (Tmult t1' t2')
+  | Tlet t1 b =>
+    t1' <- sub_t v t t1 ;;
+    y <- t_open_bound b ;;
+    let (x, t2) := y : var * tm in
+    sub_t x t t2
+  end.
+
+
+
+    Definition t_open_bound (b: tm_bound) : ctr (var * tm) :=
+  let (v, t) := b in
+  v1 <- rename_var v ;;
+  st_ret (v1, tm_subst_unsafe v (Tvar v1) t).
+  
+  Tadd (sub_t)
+
+
+
+Print fmla.
+
+
+
+(*let with bindings*)
+
+
+
+Print fmla.
+
+Print tm.
+
+
+
+
+(*Open and Close Binders*)
 
 (*TODO: implement open, close binders*)
 
